opentheory/examples/word10.ml
@@ -1,0 +1,24 @@
+(* ------------------------------------------------------------------------- *)
+(* A type of 10-bit words.                                                   *)
+(* ------------------------------------------------------------------------- *)
+
+logfile "word10-def";;
+
+let word10_width_def = new_definition
+  `word10_width = 10`;;
+
+export_thm word10_width_def;;
+
+logfile_end ();;
+
+(* Parametric theory instantiation: word *)
+
+loads "opentheory/examples/word10-word.ml";;
+
+logfile "word10-bits";;
+
+let word10_list_cases = prove_word10_list_cases 10;;
+
+export_thm word10_list_cases;;
+
+logfile_end ();;
