opentheory/haskell/all.ml
@@ -4,6 +4,8 @@
 
 start_logging ();;
 
+(***
 loads "opentheory/haskell/parser.ml";;
+***)
 
 stop_logging ();;
