opentheory/examples/word10-word.ml
@@ -1,0 +1,495 @@
+(* word10 *)
+
+(* word10-def *)
+
+new_constant ("word10_size", `:num`);;
+
+let word10_size_def = new_axiom
+  `word10_size = 2 EXP word10_width`;;
+
+let word10_size_nonzero = new_axiom
+  `~(word10_size = 0)`;;
+
+(* word10 *)
+
+(* word10-mod *)
+
+let mod_lt_word10_size = new_axiom
+  `!n. n < word10_size ==> n MOD word10_size = n`;;
+
+let lt_mod_word10_size = new_axiom
+  `!n. n MOD word10_size < word10_size`;;
+
+let mod_mod_refl_word10_size = new_axiom
+  `!n. n MOD word10_size MOD word10_size = n MOD word10_size`;;
+
+let mod_add_mod_word10_size = new_axiom
+  `!m n. (m MOD word10_size + n MOD word10_size) MOD word10_size = (m + n) MOD word10_size`;;
+
+let mod_mult_mod2_word10_size = new_axiom
+  `!m n. (m MOD word10_size * n MOD word10_size) MOD word10_size = (m * n) MOD word10_size`;;
+
+(* word10-def *)
+
+new_type ("word10",0);;
+
+new_constant ("num_to_word10", `:num -> word10`);;
+
+new_constant ("word10_to_num", `:word10 -> num`);;
+
+let word10_to_num_to_word10 = new_axiom
+  `!x. num_to_word10 (word10_to_num x) = x`;;
+
+let num_to_word10_inj = new_axiom
+   `!x y.
+      x < word10_size /\ y < word10_size /\ num_to_word10 x = num_to_word10 y ==>
+      x = y`;;
+
+let num_to_word10_to_num = new_axiom
+  `!x. word10_to_num (num_to_word10 x) = x MOD word10_size`;;
+
+new_constant ("word10_add", `:word10 -> word10 -> word10`);;
+
+let num_to_word10_add = new_axiom
+  `!x1 y1.
+     num_to_word10 (x1 + y1) =
+     word10_add (num_to_word10 x1) (num_to_word10 y1)`;;
+
+new_constant ("word10_mult", `:word10 -> word10 -> word10`);;
+
+let num_to_word10_mult = new_axiom
+  `!x1 y1.
+     num_to_word10 (x1 * y1) =
+     word10_mult (num_to_word10 x1) (num_to_word10 y1)`;;
+
+new_constant ("word10_neg", `:word10 -> word10`);;
+
+let word10_neg_def = new_axiom
+  `!x. word10_neg x = num_to_word10 (word10_size - word10_to_num x)`;;
+
+new_constant ("word10_sub", `:word10 -> word10 -> word10`);;
+
+let word10_sub_def = new_axiom
+  `!x y. word10_sub x y = word10_add x (word10_neg y)`;;
+
+new_constant ("word10_le", `:word10 -> word10 -> bool`);;
+
+let word10_le_def = new_axiom
+  `!x y. word10_le x y = word10_to_num x <= word10_to_num y`;;
+
+new_constant ("word10_lt", `:word10 -> word10 -> bool`);;
+
+let word10_lt_def = new_axiom
+  `!x y. word10_lt x y = ~(word10_le y x)`;;
+
+(* word10-thm *)
+
+let word10_to_num_inj = new_axiom
+  `!x y. word10_to_num x = word10_to_num y ==> x = y`;;
+
+let num_to_word10_eq = new_axiom
+   `!x y.
+      num_to_word10 x = num_to_word10 y <=> x MOD word10_size = y MOD word10_size`;;
+
+let word10_to_num_bound = new_axiom
+  `!x. word10_to_num x < word10_size`;;
+
+let word10_to_num_div_bound = new_axiom
+  `!x. word10_to_num x DIV word10_size = 0`;;
+
+let word10_add_to_num = new_axiom
+   `!x y.
+      word10_to_num (word10_add x y) =
+      (word10_to_num x + word10_to_num y) MOD word10_size`;;
+
+let word10_lt_alt = new_axiom
+   `!x y. word10_lt x y = word10_to_num x < word10_to_num y`;;
+
+(* word10-bits-def *)
+
+new_constant ("word10_shl", `:word10 -> num -> word10`);;
+
+let word10_shl_def = new_axiom
+  `!w n. word10_shl w n = num_to_word10 ((2 EXP n) * word10_to_num w)`;;
+
+new_constant ("word10_shr", `:word10 -> num -> word10`);;
+
+let word10_shr_def = new_axiom
+  `!w n. word10_shr w n = num_to_word10 (word10_to_num w DIV (2 EXP n))`;;
+
+new_constant ("word10_bit", `:word10 -> num -> bool`);;
+
+let word10_bit_def = new_axiom
+  `!w n. word10_bit w n = ODD (word10_to_num (word10_shr w n))`;;
+
+new_constant ("word10_to_list", `:word10 -> bool list`);;
+
+let word10_to_list_def = new_axiom
+  `!w. word10_to_list w = MAP (word10_bit w) (interval 0 word10_width)`;;
+
+new_constant ("list_to_word10", `:bool list -> word10`);;
+
+let list_to_word10_def = new_axiom
+  `(list_to_word10 [] = num_to_word10 0) /\
+   (!h t.
+      list_to_word10 (CONS h t) =
+      if h then word10_add (word10_shl (list_to_word10 t) 1) (num_to_word10 1)
+      else word10_shl (list_to_word10 t) 1)`;;
+
+new_constant ("is_word10_list", `:bool list -> bool`);;
+
+let is_word10_list_def = new_axiom
+  `!l. is_word10_list (l : bool list) <=> LENGTH l = word10_width`;;
+
+new_constant ("word10_and", `:word10 -> word10 -> word10`);;
+
+let word10_and_def = new_axiom
+  `!w1 w2.
+     word10_and w1 w2 =
+     list_to_word10 (zipwith ( /\ ) (word10_to_list w1) (word10_to_list w2))`;;
+
+new_constant ("word10_or", `:word10 -> word10 -> word10`);;
+
+let word10_or_def = new_axiom
+  `!w1 w2.
+     word10_or w1 w2 =
+     list_to_word10 (zipwith ( \/ ) (word10_to_list w1) (word10_to_list w2))`;;
+
+new_constant ("word10_not", `:word10 -> word10`);;
+
+let word10_not_def = new_axiom
+  `!w. word10_not w = list_to_word10 (MAP (~) (word10_to_list w))`;;
+
+new_constant ("word10_bits_lte", `:bool -> bool list -> bool list -> bool`);;
+
+let word10_bits_lte_def = new_axiom
+   `(!q. word10_bits_lte q [] [] = q) /\
+    (!q h1 h2 t1 t2.
+       word10_bits_lte q (CONS h1 t1) (CONS h2 t2) =
+       word10_bits_lte ((~h1 /\ h2) \/ (~(h1 /\ ~h2) /\ q)) t1 t2)`;;
+
+(* word10-bits-thm *)
+
+let length_word10_to_list = new_axiom
+  `!w. LENGTH (word10_to_list w) = word10_width`;;
+
+let is_word10_to_list = new_axiom
+  `!w. is_word10_list (word10_to_list w)`;;
+
+let word10_bit_div = new_axiom
+  `!w n. word10_bit w n = ODD (word10_to_num w DIV (2 EXP n))`;;
+
+let nil_to_word10_to_num = new_axiom
+  `word10_to_num (list_to_word10 []) = 0`;;
+
+let cons_to_word10_to_num = new_axiom
+   `!h t.
+      word10_to_num (list_to_word10 (CONS h t)) =
+      (2 * word10_to_num (list_to_word10 t) + (if h then 1 else 0)) MOD word10_size`;;
+
+let list_to_word10_to_num_bound = new_axiom
+  `!l. word10_to_num (list_to_word10 l) < 2 EXP (LENGTH l)`;;
+
+let list_to_word10_to_num_bound_suc = new_axiom
+  `!l. 2 * word10_to_num (list_to_word10 l) + 1 < 2 EXP (SUC (LENGTH l))`;;
+
+let cons_to_word10_to_num_bound = new_axiom
+   `!h t.
+      2 * word10_to_num (list_to_word10 t) + (if h then 1 else 0) <
+      2 EXP SUC (LENGTH t)`;;
+
+let word10_to_list_to_word10 = new_axiom
+  `!w. list_to_word10 (word10_to_list w) = w`;;
+
+let word10_to_list_inj = new_axiom
+  `!w1 w2. word10_to_list w1 = word10_to_list w2 ==> w1 = w2`;;
+
+let word10_to_list_inj_eq = new_axiom
+  `!w1 w2. word10_to_list w1 = word10_to_list w2 <=> w1 = w2`;;
+
+let list_to_word10_bit = new_axiom
+   `!l n.
+      word10_bit (list_to_word10 l) n =
+      (n < word10_width /\ n < LENGTH l /\ EL n l)`;;
+
+let short_list_to_word10_to_list = new_axiom
+   `!l.
+      LENGTH l <= word10_width ==>
+      word10_to_list (list_to_word10 l) =
+      APPEND l (REPLICATE (word10_width - LENGTH l) F)`;;
+
+let long_list_to_word10_to_list = new_axiom
+   `!l.
+      word10_width <= LENGTH l ==>
+      word10_to_list (list_to_word10 l) = take word10_width l`;;
+
+let list_to_word10_to_list_eq = new_axiom
+   `!l.
+      word10_to_list (list_to_word10 l) =
+      if LENGTH l <= word10_width then
+        APPEND l (REPLICATE (word10_width - LENGTH l) F)
+      else
+        take word10_width l`;;
+
+let list_to_word10_to_list = new_axiom
+  `!l. LENGTH l = word10_width <=> word10_to_list (list_to_word10 l) = l`;;
+
+let word10_shl_list = new_axiom
+   `!l n.
+      word10_shl (list_to_word10 l) n =
+      list_to_word10 (APPEND (REPLICATE n F) l)`;;
+
+let short_word10_shr_list = new_axiom
+   `!l n.
+      LENGTH l <= word10_width ==>
+      word10_shr (list_to_word10 l) n =
+      (if LENGTH l <= n then list_to_word10 []
+       else list_to_word10 (drop n l))`;;
+
+let long_word10_shr_list = new_axiom
+   `!l n.
+      word10_width <= LENGTH l ==>
+      word10_shr (list_to_word10 l) n =
+      if word10_width <= n then list_to_word10 []
+      else list_to_word10 (drop n (take word10_width l))`;;
+
+let word10_shr_list = new_axiom
+   `!l n.
+      word10_shr (list_to_word10 l) n =
+      (if LENGTH l <= word10_width then
+         if LENGTH l <= n then list_to_word10 []
+         else list_to_word10 (drop n l)
+       else
+         if word10_width <= n then list_to_word10 []
+         else list_to_word10 (drop n (take word10_width l)))`;;
+
+let word10_eq_bits = new_axiom
+  `!w1 w2. (!i. i < word10_width ==> word10_bit w1 i = word10_bit w2 i) ==> w1 = w2`;;
+
+let num_to_word10_cons = new_axiom
+  `!n.
+     list_to_word10 (CONS (ODD n) (word10_to_list (num_to_word10 (n DIV 2)))) =
+     num_to_word10 n`;;
+
+let num_to_word10_list = new_axiom
+  `!n.
+     num_to_word10 n =
+     list_to_word10
+       (if n = 0 then []
+        else CONS (ODD n) (word10_to_list (num_to_word10 (n DIV 2))))`;;
+
+let word10_lte_list = new_axiom
+   `!q w1 w2.
+      word10_bits_lte q (word10_to_list w1) (word10_to_list w2) <=>
+      (if q then word10_le w1 w2 else word10_lt w1 w2)`;;
+
+let word10_le_list = new_axiom
+   `!w1 w2.
+      word10_bits_lte T (word10_to_list w1) (word10_to_list w2) <=> word10_le w1 w2`;;
+
+let word10_lt_list = new_axiom
+   `!w1 w2.
+      word10_bits_lte F (word10_to_list w1) (word10_to_list w2) <=> word10_lt w1 w2`;;
+
+let word10_reduce_conv =
+    REWRITE_CONV
+      [word10_to_num_to_word10;
+       word10_le_def; word10_lt_def] THENC
+    REWRITE_CONV
+      [num_to_word10_to_num] THENC
+    REWRITE_CONV
+      [word10_width_def; word10_size_def; num_to_word10_eq] THENC
+    NUM_REDUCE_CONV;;
+
+let word10_width_conv = REWR_CONV word10_width_def;;
+
+let list_to_word10_to_list_conv =
+    REWR_CONV list_to_word10_to_list_eq THENC
+    cond_conv
+      (RATOR_CONV (RAND_CONV length_conv) THENC
+       RAND_CONV word10_width_conv THENC
+       NUM_REDUCE_CONV)
+      (RAND_CONV
+         ((RATOR_CONV o RAND_CONV)
+            (RATOR_CONV (RAND_CONV word10_width_conv) THENC
+             RAND_CONV length_conv THENC
+             NUM_REDUCE_CONV) THENC
+          replicate_conv) THENC
+       append_conv)
+      (RATOR_CONV (RAND_CONV word10_width_conv) THENC
+       take_conv);;
+
+let numeral_to_word10_list_conv =
+    let zero_conv = REWR_CONV (SYM (CONJUNCT1 list_to_word10_def)) in
+    let numeral_conv = REWR_CONV (SYM (SPEC `NUMERAL n` num_to_word10_cons)) in
+    let rec rewr_conv tm =
+        (zero_conv ORELSEC
+         (numeral_conv THENC
+          RAND_CONV
+            (RATOR_CONV (RAND_CONV NUM_REDUCE_CONV) THENC
+             RAND_CONV
+               (RAND_CONV
+                  (RAND_CONV NUM_REDUCE_CONV THENC
+                   rewr_conv) THENC
+                list_to_word10_to_list_conv)))) tm in
+    rewr_conv;;
+
+let word10_and_list_conv =
+    let th = SPECL [`list_to_word10 l1`; `list_to_word10 l2`] word10_and_def in
+    REWR_CONV th THENC
+    RAND_CONV
+      (RATOR_CONV (RAND_CONV list_to_word10_to_list_conv) THENC
+       RAND_CONV list_to_word10_to_list_conv THENC
+       zipwith_conv and_simp_conv);;
+
+let word10_or_list_conv =
+    let th = SPECL [`list_to_word10 l1`; `list_to_word10 l2`] word10_or_def in
+    REWR_CONV th THENC
+    RAND_CONV
+      (RATOR_CONV (RAND_CONV list_to_word10_to_list_conv) THENC
+       RAND_CONV list_to_word10_to_list_conv THENC
+       zipwith_conv or_simp_conv);;
+
+let word10_shr_list_conv =
+    let th = SPECL [`l : bool list`; `NUMERAL n`] word10_shr_list in
+    REWR_CONV th THENC
+    cond_conv
+      (RATOR_CONV (RAND_CONV length_conv) THENC
+       RAND_CONV word10_width_conv THENC
+       NUM_REDUCE_CONV)
+      (cond_conv
+        (RATOR_CONV (RAND_CONV length_conv) THENC
+         NUM_REDUCE_CONV)
+        ALL_CONV
+        (RAND_CONV drop_conv))
+      (cond_conv
+        (RATOR_CONV (RAND_CONV word10_width_conv) THENC
+         NUM_REDUCE_CONV)
+        ALL_CONV
+        (RAND_CONV
+           (RAND_CONV
+              (RATOR_CONV (RAND_CONV word10_width_conv) THENC
+               take_conv) THENC
+            drop_conv)));;
+
+let word10_shl_list_conv =
+    let th = SPECL [`l : bool list`; `NUMERAL n`] word10_shl_list in
+    REWR_CONV th THENC
+    RAND_CONV
+      (RATOR_CONV (RAND_CONV replicate_conv) THENC
+       append_conv);;
+
+let word10_bit_list_conv =
+    let th = SPECL [`l : bool list`; `NUMERAL n`] list_to_word10_bit in
+    REWR_CONV th THENC
+    andalso_conv
+      (RAND_CONV word10_width_conv THENC
+       NUM_REDUCE_CONV)
+      (andalso_conv
+        (RAND_CONV length_conv THENC
+         NUM_REDUCE_CONV)
+        el_conv);;
+
+let word10_bits_lte_conv =
+    let nil_conv = REWR_CONV (CONJUNCT1 word10_bits_lte_def) in
+    let cons_conv = REWR_CONV (CONJUNCT2 word10_bits_lte_def) in
+    let rec rewr_conv tm =
+        (nil_conv ORELSEC
+         (cons_conv THENC
+          (RATOR_CONV o RATOR_CONV o RAND_CONV)
+            ((RATOR_CONV o RAND_CONV)
+               (RATOR_CONV (RAND_CONV (TRY_CONV not_simp_conv)) THENC
+                TRY_CONV and_simp_conv) THENC
+             RAND_CONV
+               ((RATOR_CONV o RAND_CONV)
+                  (RAND_CONV
+                    (RAND_CONV (TRY_CONV not_simp_conv) THENC
+                     TRY_CONV and_simp_conv) THENC
+                   TRY_CONV not_simp_conv) THENC
+                TRY_CONV and_simp_conv) THENC
+             TRY_CONV or_simp_conv) THENC
+          rewr_conv)) tm in
+    rewr_conv;;
+
+let word10_le_list_conv =
+    let th = SYM (SPECL [`list_to_word10 l1`; `list_to_word10 l2`] word10_le_list) in
+    REWR_CONV th THENC
+    RATOR_CONV (RAND_CONV list_to_word10_to_list_conv) THENC
+    RAND_CONV list_to_word10_to_list_conv THENC
+    word10_bits_lte_conv;;
+
+let word10_lt_list_conv =
+    let th = SYM (SPECL [`list_to_word10 l1`; `list_to_word10 l2`] word10_lt_list) in
+    REWR_CONV th THENC
+    RATOR_CONV (RAND_CONV list_to_word10_to_list_conv) THENC
+    RAND_CONV list_to_word10_to_list_conv THENC
+    word10_bits_lte_conv;;
+
+let word10_eq_list_conv =
+    let th = SYM (SPECL [`list_to_word10 l1`; `list_to_word10 l2`]
+                    word10_to_list_inj_eq) in
+    REWR_CONV th THENC
+    RATOR_CONV (RAND_CONV list_to_word10_to_list_conv) THENC
+    RAND_CONV list_to_word10_to_list_conv THENC
+    list_eq_conv iff_simp_conv;;
+
+let word10_bit_conv =
+    word10_width_conv ORELSEC
+    list_to_word10_to_list_conv ORELSEC
+    numeral_to_word10_list_conv ORELSEC
+    word10_and_list_conv ORELSEC
+    word10_or_list_conv ORELSEC
+    word10_shr_list_conv ORELSEC
+    word10_shl_list_conv ORELSEC
+    word10_bit_list_conv ORELSEC
+    word10_le_list_conv ORELSEC
+    word10_lt_list_conv ORELSEC
+    word10_eq_list_conv;;
+
+let bit_blast_subterm_conv = word10_bit_conv ORELSEC bit_blast_subterm_conv;;
+let bit_blast_conv = DEPTH_CONV bit_blast_subterm_conv;;
+let bit_blast_tac = CONV_TAC bit_blast_conv;;
+
+let prove_word10_list_cases n =
+    let interval =
+        let rec intv i n = if n = 0 then [] else i :: intv (i + 1) (n - 1) in
+        intv 0 in
+    let lemma1 =
+        let nunary = funpow n (fun t -> mk_comb (`SUC`,t)) `0` in
+        let goal = mk_eq (`LENGTH (word10_to_list w)`,nunary) in
+        let tac =
+            REWRITE_TAC [length_word10_to_list; word10_width_def] THEN
+            NUM_REDUCE_TAC in
+        prove (goal,tac) in
+    let witnesses =
+        let addtl l = mk_comb (`TL : bool list -> bool list`, hd l) :: l in
+        let tls = rev (funpow (n - 1) addtl [`l : bool list`]) in
+        map (fun t -> mk_comb (`HD : bool list -> bool`, t)) tls in
+    let goal =
+        let is = interval n in
+        let xs = map (fun i -> mk_var ("x" ^ string_of_int i, bool_ty)) is in
+        let w = mk_var ("w", `:word10`) in
+        let body = mk_eq (w, mk_comb (`list_to_word10`, mk_list (xs,bool_ty))) in
+        mk_forall (w, list_mk_exists (xs,body)) in
+    let tac =
+        GEN_TAC THEN
+        CONV_TAC
+          (funpow n (RAND_CONV o ABS_CONV)
+             (LAND_CONV (ONCE_REWRITE_CONV [GSYM word10_to_list_to_word10]))) THEN
+        MP_TAC lemma1 THEN
+        SPEC_TAC (`word10_to_list w`, `l : bool list`) THEN
+        REPEAT STRIP_TAC THEN
+        EVERY (map EXISTS_TAC witnesses) in
+        AP_TERM_TAC THEN
+        POP_ASSUM MP_TAC THEN
+        N_TAC n
+          (MP_TAC (ISPEC `l : bool list` list_CASES) THEN
+           STRIP_TAC THENL
+           [ASM_REWRITE_TAC [LENGTH; NOT_SUC];
+            ALL_TAC] THEN
+           POP_ASSUM SUBST_VAR_TAC THEN
+           REWRITE_TAC [LENGTH; SUC_INJ; HD; TL; CONS_11] THEN
+           SPEC_TAC (`t : bool list`, `l : bool list`) THEN
+           GEN_TAC) THEN
+        REWRITE_TAC [LENGTH_EQ_NIL] in
+    prove (goal,tac);;
