opentheory/stdlib/tactics.ml
@@ -42,6 +42,10 @@ let bool_simp_conv =
     iff_simp_conv ORELSEC
     cond_simp_conv;;
 
+let bit_blast_subterm_conv = bool_simp_conv;;
+let bit_blast_conv = DEPTH_CONV bit_blast_subterm_conv;;
+let bit_blast_tac = CONV_TAC bit_blast_conv;;
+
 let cond_conv =
     let pth = SPEC_ALL COND_CLAUSES in
     let ac = REWR_CONV (CONJUNCT1 pth) in
